\documentclass{article}
\usepackage[utf8]{inputenc}
\usepackage{geometry}
\usepackage{amssymb}
\usepackage{graphicx}
\usepackage{marginnote}
\usepackage{amsmath}
\usepackage{parskip}

%Document Organisation: 
\author{Zain Sikand}
\title{Problem Catalogue}
\geometry{margin=3cm}
%Starting Document:  
\begin{document}
\begin{raggedright}
%Formatting: 
\pagenumbering{arabic}
\tableofcontents 
\newpage 
\maketitle

%Section 1: 
\section{Integrals: Evil} 
\subsection{\underline{Problem One}} \par

\textbf{\emph{Problem Author: Zain Sikand}} \\
\textit{Your final answer should be a single expression in the form $I_1=[h(x)]_{a}^{b}$ where b and a are bounds of $I_1$ to be found} 
\newline \\
Conclude whether or not the below integral, $I_1:$
$$I_{1}= \int_{\int_{x}^{2x}(\ln x)^{2}}^{(3+x)^{6}}(\frac{1}{3e^{x}\cos x \sec^{2} x} + \cot x \csc x) \ dx $$
can be written as a single expression, with all integration expressions evaluated. 
\newline \\ 
{Your conclusion must be supported, \textbf{either}, by an attempt to evaluate the integral or, a proof that  $I_{1}$ has no real anti-derivative.} 
\newline \\
\quote|\textit{12 Marks}| \\
\newpage
\subsubsection{Worked Solution:}
$$I_{1} = \int_{\int_{x}^{2x}(lnx)^{2}}^{(3+x)^{6}}(\frac{1}{3e^{x}\cos x \sec^{2} x} + \cot x \csc x) \ dx $$
$\Rightarrow \ I_{1}=\int_{b}^{a} f(x) dx$ \\

$\therefore \ let \ I_{2}=b$ \\
$$I_2=\int_{x}^{2x}(\ln|x|)^{2}= \int^{2e^{u}}_{e^{u}}u^{2}e^{u}du=[u^{2}e^{u}]^{2e^{u}}_{e^{u}}-\int^{2e^{u}}_{e^{u}}2ue^{u}e^{u}du$$ \\
$$= [u^{2}e^{u}]^{2e^{u}}_{e^{u}}- ([2ue^{u}]^{2e^{u}}_{e^{u}}- \int ^{2e^{u}}_{e^{u}}2e^{u}du=[u^{2}e^{u}] ^{2e^{u}}_{e^{u}}-[2ue^{u}-2e^{u}]^{2e^{u}}_{e^{u}}=[u^{2}e^{u}-2ue^{u}-2e^{u}]^{2e^{u}}_{e^{u}}$$ \\
$$=[x(\ln |x|)^{2}-2x\ln|x|-2x]^{2x}_{x} \because u=\ln|x| \Rightarrow e^{u}=x $$ \\
$\therefore I_2=x[2(\ln |2x|)^{2}-(\ln |x|)^{2}-\ln |16x^{2}|]$ \marginnote{This result can be obtained by evaluating the bounds} \\
$$I_1= \int^{(3+x)^{6}}_{I_{2}} (\frac{1}{3e^{x}\cos x \sec^{2} x} + \cot x \csc x) \ dx = \int^b_a(\frac{1}{3e^{x}\cos x \sec^{2} x)} + \int^{b}_{a} \cot x \csc x$$ \\
$$let \ I_{3}= \int^b_a(\frac{1}{3e^{x}\cos x \sec^{2} x)} = \int^b_a(\frac{1}{3e^{x}\sec x)}dx = \frac{1}{3} \int^b_a(e^{-x}\cos x)dx$$ \\
$$I_{3}=1/3(J) $$ \\
$$J=[-e^{-x}\cos x]^b_a - \int^b_a -e^{-x}\sin x = [-e^{-x}\cos x]^b_a-([-e^{-x}\sin x]^b_a-\int^b_ae^{-x}cosx$$ \\
$$J=[-e^{-x}\cos x]^b_a-[e^{-x}\sin x]^b_a-J $$ \\
$$\therefore \ J=\frac{1}{2}[e^{-x}\sin x-e^{-x}\cos x]^b_a$$ \\
$$\therefore \ I_{3}=\frac{1}{6}[e^{-x}\sin x-e^{-x}\cos x]^b_a$$ \\
$$I_{1}=I_{3}+\int^b_a\cot x \csc x \ dx$$ \\
$$ let \ I_{4}= \int^b_a\cot x \csc x \ dx$$ \\
$$I_{4}= \int^b_a (\frac{1}{\sin x})(\frac{\cos x}{\sin x}) \ dx = \int^b_a \frac{\cos x}{1-\cos^{2} x} \ dx $$ \\
\textbf{Integrate $I_4$ by parts:}
$$ I_{4}=\int^b_a \frac{\cos x}{\sin^{2} x} \ dx = \int^b_a \cos x ( \frac{1}{\sin^{2} x}) \ dx = [\frac{1}{\sin x}]^b_a-\int^b_a \sin x ( \frac{-2\sin x\cos x}{\sin^{4} x}) \ dx = [\frac{1}{\sin x}]^b_a-\int^b_a \frac{-2 \cos x}{\sin x} \ dx $$ \\
$$ \therefore I_{4}= [\frac{1}{\sin x}]^b_a+ 2I_{4}$$ \\
$$\Rightarrow I_{4}=-\frac{1}{\sin x} $$
$$ \therefore I_{1}= [I_{3}+I_{4}]^b_a $$
\footnote{ \textbf{ Warning:} Solution is unverified} 
$\therefore$ The integral $I_{1}$ can be written as a single expression within its bounds 
$\therefore$ Q.E.D

\subsection{\underline{Problem 2}}

\end{raggedright} 
\end{document}