\documentclass{article}
% Allow the usage of UTF-8 characters
\usepackage[utf8]{inputenc}
\usepackage{geometry}
\usepackage{amssymb}
% Allow the usage of graphics (.png, .jpg)
\usepackage{graphicx}
\author{Zain Sikand}
\title{Zain's Problem Catalogue}
\geometry{margin=3cm} 
\usepackage{marginnote}
% Start the document
\begin{document}
\begin{raggedright}
\pagenumbering{arabic}
\tableofcontents 
\newpage 
\maketitle
\section{Integrals: Evil} 
\subsection{\underline{Problem One}}
by \textbf{Zain Sikand} \\
\textit{Your final answer should be a single expression in the form $I_1=[h(x)]_{a}^{b}$ where b and a are bounds of $I_1$ to be found} 
\newline \\
Conclude whether or not the below integral $I_1$, can be written as a single expression, with all integration expressions evaluated. \\
{Your conclusion must be supported, either, by an attempt to evaluate the integral or, a proof that  $I_{1}$ has no real anti-derivative.}
$$
I_{1}= \int_{\int_{x}^{2x}(\ln x)^{2}}^{(3+x)^{6}}(\frac{1}{3e^{x}\cos x \sec^{2} x} + \cot x \csc x) \ dx 
$$

\newpage
\subsubsection{Worked Solution:}

$$
I_{1}= \int_{\int_{x}^{2x}(lnx)^{2}}^{(3+x)^{6}}(\frac{1}{3e^{x}\cos x \sec^{2} x} + \cot x \csc x) \ dx 
$$
$\Rightarrow \ I_{1}=\int_{b}^{a} f(x) dx$ \\

$\therefore \ let \ I_{2}=b$
$$
I_2=\int_{x}^{2x}(\ln|x|)^{2}= \int^{2e^{u}}_{e^{u}}u^{2}e^{u}du=[u^{2}e^{u}]^{2e^{u}}_{e^{u}}-\int^{2e^{u}}_{e^{u}}2ue^{u}e^{u}du
$$
\\
$$
= [u^{2}e^{u}]^{2e^{u}}_{e^{u}}- ([2ue^{u}]^{2e^{u}}_{e^{u}}- \int ^{2e^{u}}_{e^{u}}2e^{u}du=[u^{2}e^{u}] ^{2e^{u}}_{e^{u}}-[2ue^{u}-2e^{u}]^{2e^{u}}_{e^{u}}=[u^{2}e^{u}-2ue^{u}-2e^{u}]^{2e^{u}}_{e^{u}}$$
\\
$$
=[x(\ln |x|)^{2}-2x\ln|x|-2x]^{2x}_{x} \because u=\ln|x| \Rightarrow e^{u}=x 
$$
\\
$\therefore I_2=x[2(\ln |2x|)^{2}-(\ln |x|)^{2}-\ln |16x^{2}|]$ \marginnote{This result can be obtained by evaluating the bounds} 
\\
$$ 
I_1= \int^{(3+x)^{6}}_{I_{2}} (\frac{1}{3e^{x}\cos x \sec^{2} x} + \cot x \csc x) \ dx = \int^b_a(\frac{1}{3e^{x}\cos x \sec^{2} x)} + \int^{b}_{a} \cot x \csc x
$$
\\
$$
let \ I_{3}= \int^b_a(\frac{1}{3e^{x}\cos x \sec^{2} x)}= \int^b_a(\frac{1}{3e^{x}\sec x)}dx= \frac{1}{3} \int^b_a(e^{-x}\cos x)dx$$
\\
$$
I_{3}=1/3(J) 
$$ 
\\
$$
J=[-\cos xe^{-x}]^b_a - \int^b_a -e^{-x}\sin x = [-e^{-x}\cos x]^b_a-([-e^{-x}\sin x]^b_a-\int^b_ae^{-x}cosx
$$
\\
$$
J=[-e^{-x}\cos x]^b_a-[e^{-x}\sin x]^b_a-J 
$$
\\
$$
\therefore \ J=\frac{1}{2}[e^{-x}\sin x-e^{-x}\cos x]^b_a
$$
\\
$$
\therefore \ I_{3}=\frac{1}{6}[e^{-x}\sin x-e^{-x}\cos x]^b_a
$$
\\
$$
I_{1}=I_{3}+\int^b_a\cot x \csc x \ dx
$$
\\
$$ 
let \ I_{4}= \int^b_a\cot x \csc x \ dx$$

$$I_{4}= \int^b_a (\frac{1}{\sin x})(\frac{\cos x}{\sin x}) \ dx = \int^b_a \frac{\cos x}{1-\cos^{2} x} \ dx 
$$
\\
\textbf{Integrate $I_4$ by parts:}
$$
I_{4}=\int^b_a \frac{\cos x}{\sin^{2} x} \ dx = \int^b_a \cos x ( \frac{1}{\sin^{2} x}) \ dx = [\frac{1}{\sin x}]^b_a-\int^b_a \sin x ( \frac{-2\sin x\cos x}{\sin^{4} x}) \ dx = [\frac{1}{\sin x}]^b_a-\int^b_a \frac{-2 \cos x}{\sin x} \ dx 
$$
\\
$$ 
\therefore I_{4}= [\frac{1}{\sin x}]^b_a+ 2I_{4}
$$
\\
$$
\Rightarrow I_{4}=-\frac{1}{\sin x} 
$$
$$ 
\therefore I_{1}= [I_{3}+I_{4}]^b_a 
$$
\footnote{ \textbf{ Warning:} Solution is unverified} 
$\therefore$ The integral $I_{1}$ can be written as a single expression within its bounds 
$\therefore$ Q.E.D
\end{raggedright} 
\end{document}